fstar/new/CryptoMLS.fst
@@ -1,0 +1,47 @@
+module CryptoMLS
+
+include Crypto
+open Lib.Result
+open Parser
+open Lib.IntTypes
+open Lib.ByteSequence
+
+noeq type kdf_label_nt = {
+  kln_length: uint16;
+  kln_label: blbytes ({min=7; max=255});
+  kln_context: blbytes ({min=0; max=(pow2 32)-1});
+}
+
+val ps_kdf_label: parser_serializer kdf_label_nt
+let ps_kdf_label =
+  isomorphism kdf_label_nt
+    (
+      _ <-- ps_u16;
+      _ <-- ps_bytes _;
+      ps_bytes _
+    )
+    (fun (|length, (|label, context|)|) -> {kln_length=length; kln_label=label; kln_context=context;})
+    (fun x -> (|x.kln_length, (|x.kln_label, x.kln_context|)|))
+
+val expand_with_label: ciphersuite -> secret:bytes -> label:bytes -> context:bytes -> len:size_nat -> result (lbytes len)
+let expand_with_label cs secret label context len =
+  assert_norm (String.strlen "mls10 " == 6);
+  if not (len < pow2 16) then
+    fail "expand_with_label: len too high"
+  else if not (1 <= Seq.length label) then
+    fail "expand_with_label: label too short"
+  else if not (Seq.length label < 255-6) then
+    fail "expand_with_label: label too long"
+  else if not (Seq.length context < pow2 32) then
+    fail "expand_with_label: context too long"
+  else
+    let kdf_label = ps_kdf_label.serialize ({
+      kln_length = u16 len;
+      kln_label = Seq.append (string_to_bytes "mls10 ") label;
+      kln_context = context;
+    }) in
+    kdf_expand cs secret kdf_label len
+
+val derive_secret: cs:ciphersuite -> secret:bytes -> label:bytes -> result (lbytes (kdf_length cs))
+let derive_secret cs secret label =
+  expand_with_label cs secret label bytes_empty (kdf_length cs)
